sadfsdaf

Hashtable.dfy
@@ -31,14 +31,14 @@ class Hashtable<K(==,!new),V(!new)> {
   //2. The hastable and its contents implement exactly a map
   ghost predicate valid_data(k:K,v:V,m:map<K,Option<V>>, d:array<List<(K,V)>>)
     reads this, d
-    requires 0 < size == d.Length
+    requires 0 < d.Length
   {
-    var b := bucket(k, size);
+    var b := bucket(k, d.Length);
     (k in m && m[k] == Some(v)) ==> mem((k,v), d[b]) && (k !in m) ==> !mem((k,v), d[b])
   }
   ghost predicate valid_map()
     reads this, data
-    requires 0 < size == data.Length
+    requires 0 < data.Length
   {
     forall k, v :: valid_data(k,v,mapa,data)
   }
@@ -46,7 +46,7 @@ class Hashtable<K(==,!new),V(!new)> {
   ghost predicate valid()
     reads this, data
   {
-    0 < size == data.Length && valid_pairs_bucket() && valid_map()
+    0 < data.Length && valid_pairs_bucket() && valid_map()
   }
 
   function hash(key: K) : int
@@ -59,11 +59,11 @@ class Hashtable<K(==,!new),V(!new)> {
 
   constructor(n: int)
     requires n > 0
-    ensures 0 < size == data.Length
+    ensures 0 < data.Length
     ensures valid()
     ensures mapa == map[] && fresh(data)
   {
-    size := n;
+    size := 0;
     data := new List<(K,V)>[n](_ => Nil);
     mapa := map[];
   }
@@ -78,17 +78,57 @@ class Hashtable<K(==,!new),V(!new)> {
     var i:int := 0;
     var new_data := new List<(K,V)>[data.Length](_ => Nil);
     data := new_data;
+    size := 0;
+  }
+
+  method rehash(arr: array<List<(K,V)>>, l : List<(K,V)>, index : int)
+    requires valid()
+    requires 0 <= index < arr.Length
+    modifies this, arr
+    ensures valid_hash(arr, index)
+  {
+    match l
+    case Nil => {}
+    case Cons((k, v), xs) => {
+      var b := bucket(k, arr.Length);
+      arr[b] := Cons((k,v), arr[b]);
+      mapa := mapa[k := Some(v)];
+      rehash(arr, xs, index);
+    }
   }
 
   method resize()
-
-  function mem<T(==)> (k: T, l: List<T>) : bool
+    requires valid()
+    modifies this, data
+    ensures valid()
+    ensures fresh(data)
   {
-    match l
-    case Nil => false
-    case Cons(k', t) =>
-      if(k' == k) then true else mem(k, t)
+    var new_length := data.Length * 2;
+    var new_data := new List<(K,V)>[new_length](_ => Nil);
+    var i:int := 0;
+    while(i < data.Length)
+      invariant 0 <= i <= data.Length
+      invariant valid_hash(new_data, i)
+      modifies new_data
+    {
+      rehash(new_data, data[i], i);
+      i := i + 1;
+    }
+    data := new_data;
   }
+
+  ghost function mem<T>(x:T, l:List<T>) : bool {
+    match l {
+      case Nil => false
+      case Cons(y,xs) => x==y || mem(x,xs)
+    }
+  }
+
+  ghost function length<T>(l:List<T>) : int {
+    match l {
+      case Nil => 0
+      case Cons(_,xs) => 1 + length(xs)
+    } }
 
   function list_find (k:K, l:List<(K,V)>) : Option<V>
     ensures match list_find(k,l) {
@@ -106,35 +146,44 @@ class Hashtable<K(==,!new),V(!new)> {
     requires valid()
     ensures valid()
     ensures match r {
-              case None => forall v :: !mem((k,v),data[bucket(k,size)])
-              case Some(v) => mem((k,v),data[bucket(k,size)])
+              case None => forall v :: !mem((k,v),data[bucket(k,data.Length)])
+              case Some(v) => mem((k,v),data[bucket(k,data.Length)])
             }
   {
-    var b := bucket(k, size);
+    var b := bucket(k, data.Length);
     r := list_find(k, data[b]);
   }
 
-  function list_remove(k: K,l: List<(K,V)>) : List<(K,V)>
+
+  function list_remove<K(==,!new),V(!new)>(k:K,l:List<(K,V)>) : List<(K,V)>
     decreases l
-    ensures forall k' , v :: mem((k',v),list_remove(k,l)) <==> (mem((k',v),l) && k' != k)
+    ensures forall k' , v :: mem((k',v),list_remove(k,l)) <==>
+                             (mem((k',v),l) && k != k')
   {
     match l {
       case Nil => Nil
       case Cons((k',v),xs) => if k==k' then list_remove(k,xs) else
       Cons((k',v),list_remove(k,xs))
-    }
-  }
+    } }
 
   method remove(k: K)
     modifies this, data
     requires valid()
     ensures valid()
     ensures k !in mapa
-    ensures forall v :: !mem((k,v),data[bucket(k,size)])
+    ensures forall v :: !mem((k,v),data[bucket(k,data.Length)])
   {
-    var b := bucket(k, size);
+    var kExists := find(k);
+    if(kExists != None) {
+      size := size - 1;
+    }
+    var b := bucket(k, data.Length);
+    assert valid_hash_aux(data.Length, data[b], b);
     data[b] := list_remove(k, data[b]);
     mapa := mapa - {k};
+    assert valid_hash_aux(data.Length, old(data)[b], b);
+    assert bucket(k, data.Length) == b;
+    assert old(data).Length == data.Length;
   }
 
   method add(k: K,v: V)
@@ -142,9 +191,13 @@ class Hashtable<K(==,!new),V(!new)> {
     requires valid()
     ensures valid()
     ensures k in mapa ==> mapa[k] == Some(v)
-    ensures mem((k,v), data[bucket(k,size)])
+    ensures mem((k,v), data[bucket(k,data.Length)])
   {
-    var b := bucket(k, size);
+    var kExists := find(k);
+    if(kExists == None) {
+      size := size + 1;
+    }
+    var b := bucket(k, data.Length);
     data[b] := Cons((k,v), data[b]);
     mapa := mapa[k := Some(v)];
   }
